src/ListLemmas.v
@@ -5,6 +5,8 @@ Import ListNotations.
 Require Import Monads.
 
 
+(* nat <= *)
+
 Lemma nat_max_le : forall n1 n2 m,
     max n1 n2 <= m ->
     n1 <= m /\ n2 <= m.
@@ -26,6 +28,8 @@ Lemma nat_le_max : forall n1 n2 m,
 intros0 Hle1 Hle2. destruct (Max.max_spec n1 n2) as [[? ?] | [? ?]]; omega.
 Qed.
 
+
+(* maximum *)
 
 Fixpoint maximum ns :=
     match ns with
@@ -50,6 +54,8 @@ Lemma maximum_le_Forall : forall ns m,
 intros; split; eauto using maximum_le_Forall_fwd, maximum_le_Forall_rev.
 Qed.
 
+
+(* map_partial *)
 
 Fixpoint map_partial {A B : Type} (f : A -> option B) (l : list A) : option (list B) :=
   match l with
@@ -94,6 +100,79 @@ induction xs; inversion 1; subst; simpl in *.
 - find_rewrite. erewrite IHxs by eauto. reflexivity.
 Qed.
 
+Lemma map_partial_cons : forall A B (f : A -> option B) x xs y ys,
+    f x = Some y ->
+    map_partial f xs = Some ys ->
+    map_partial f (x :: xs) = Some (y :: ys).
+intros0 Hx Hxs. simpl. repeat find_rewrite. reflexivity.
+Qed.
+
+Lemma map_partial_app : forall A B (f : A -> option B) xs1 xs2 ys1 ys2,
+    map_partial f xs1 = Some ys1 ->
+    map_partial f xs2 = Some ys2 ->
+    map_partial f (xs1 ++ xs2) = Some (ys1 ++ ys2).
+induction xs1; destruct ys1; intros0 Hxs1 Hxs2; simpl in * |-;
+repeat (break_match; try discriminate); try discriminate.
+- eauto.
+- inject_some. specialize (IHxs1 xs2 ?? ?? *** **).
+  repeat rewrite <- app_comm_cons in *. repeat find_rewrite.
+  eapply map_partial_cons; eassumption.
+Qed.
+
+Lemma map_partial_cons_inv : forall A B (f : A -> option B) x1 xs2 ys
+        (P : _ -> _ -> _ -> Prop),
+    (forall y1 ys2,
+        f x1 = Some y1 ->
+        map_partial f xs2 = Some ys2 ->
+        ys = y1 :: ys2 ->
+        P x1 xs2 ys) ->
+    map_partial f (x1 :: xs2) = Some ys -> P x1 xs2 ys.
+intros0 HQ Hmap.
+simpl in Hmap. repeat (break_match; try discriminate).
+inject_some. eauto.
+Qed.
+
+Lemma map_partial_app_inv : forall A B (f : A -> option B) xs1 xs2 ys
+        (P : _ -> _ -> _ -> Prop),
+    (forall ys1 ys2,
+        map_partial f xs1 = Some ys1 ->
+        map_partial f xs2 = Some ys2 ->
+        ys = ys1 ++ ys2 ->
+        P xs1 xs2 ys) ->
+    map_partial f (xs1 ++ xs2) = Some ys -> P xs1 xs2 ys.
+induction xs1; intros0 HQ Hmap; simpl in Hmap.
+- simpl in HQ. eauto. 
+- repeat (break_match; try congruence). inject_some.
+  inversion Heqo0 using (IHxs1 xs2 l).
+  intros. subst. eapply HQ.
+  + simpl. repeat find_rewrite. reflexivity.
+  + eassumption.
+  + reflexivity.
+Qed.
+
+Lemma map_partial_3part_inv : forall A B (f : A -> option B) xs1 x2 xs3 ys
+        (P : _ -> _ -> _ -> _ -> Prop),
+    (forall ys1 y2 ys3,
+        map_partial f xs1 = Some ys1 ->
+        f x2 = Some y2 ->
+        map_partial f xs3 = Some ys3 ->
+        ys = ys1 ++ y2 :: ys3 ->
+        P xs1 x2 xs3 ys) ->
+    map_partial f (xs1 ++ x2 :: xs3) = Some ys -> P xs1 x2 xs3 ys.
+intros0 HQ Hmap.
+on _, invc_using map_partial_app_inv.
+on _, invc_using map_partial_cons_inv.
+eauto.
+Qed.
+
+Lemma map_partial_length : forall A B (f : A -> option B) xs ys,
+    map_partial f xs = Some ys ->
+    length xs = length ys.
+intros0 Hmap. eapply map_partial_Forall2 in Hmap. eauto using Forall2_length.
+Qed.
+
+
+(* Forall / Forall2 *)
 
 Lemma Forall_map : forall A B (P : B -> Prop) (f : A -> B) xs,
     Forall (fun x => P (f x)) xs <-> Forall P (map f xs).
@@ -101,3 +180,68 @@ induction xs; intros; split; inversion 1; subst; simpl in *; eauto.
 - constructor; eauto. rewrite <- IHxs. assumption.
 - constructor; eauto. rewrite -> IHxs. assumption.
 Qed.
+
+Lemma Forall2_map : forall A A' B B' (P : A' -> B' -> Prop) (fx : A -> A') (fy : B -> B') xs ys,
+    Forall2 (fun x y => P (fx x) (fy y)) xs ys <-> Forall2 P (map fx xs) (map fy ys).
+induction xs; destruct ys; intros; split; inversion 1; subst; simpl in *; eauto.
+- constructor; eauto. rewrite <- IHxs. assumption.
+- constructor; eauto. rewrite -> IHxs. assumption.
+Qed.
+
+Lemma Forall2_map_eq : forall A B R (fx : A -> R) (fy : B -> R) xs ys,
+    Forall2 (fun x y => fx x = fy y) xs ys ->
+    map fx xs = map fy ys.
+induction xs; destruct ys; intros0 Hfa; invc Hfa; eauto.
+simpl. specialize (IHxs ?? **). repeat find_rewrite. reflexivity.
+Qed.
+
+Lemma Forall2_Forall_exists : forall A B (P : A -> B -> Prop) xs ys,
+    Forall2 P xs ys ->
+    Forall (fun x => exists y, P x y) xs.
+induction xs; destruct ys; intros0 Hfa; invc Hfa; eauto.
+Qed.
+
+Lemma Forall_app_inv : forall A (P : A -> Prop) xs1 xs2
+        (Q : _ -> _ -> _ -> _ -> Prop),
+    (Forall P xs1 -> Forall P xs2 -> Q A P xs1 xs2) ->
+    Forall P (xs1 ++ xs2) -> Q A P xs1 xs2.
+induction xs1; intros0 HQ Hfa.
+- eauto.
+- rewrite <- app_comm_cons in *. invc Hfa.
+  on _, invc_using IHxs1. eauto.
+Qed.
+
+Lemma Forall_3part_inv : forall A (P : A -> Prop) xs1 x2 xs3
+        (Q : _ -> _ -> _ -> _ -> _ -> Prop),
+    (Forall P xs1 -> P x2 -> Forall P xs3 -> Q A P xs1 x2 xs3) ->
+    Forall P (xs1 ++ x2 :: xs3) -> Q A P xs1 x2 xs3.
+intros0 HQ Hfa.
+inversion Hfa using Forall_app_inv; intros.
+on (Forall _ (_ :: _)), invc.
+eauto.
+Qed.
+
+
+(* misc *)
+
+Lemma map_id : forall A (xs : list A), map id xs = xs.
+induction xs; unfold id in *; simpl; congruence.
+Qed.
+
+Lemma skipn_more : forall A i (xs : list A) y ys,
+    skipn i xs = y :: ys ->
+    skipn (S i) xs = ys.
+induction i; intros; simpl in *; subst.
+- reflexivity.
+- destruct xs; try discriminate. eapply IHi; eauto.
+Qed.
+
+Lemma skipn_nth_error : forall A i (xs : list A) y ys,
+    skipn i xs = y :: ys ->
+    nth_error xs i = Some y.
+induction i; intros; simpl in *; subst.
+- reflexivity.
+- destruct xs; try discriminate. eauto.
+Qed.
+
+
